δ=
  If(

    tir ∧ plzdtyA ∧ Angle(

      Incident_{2nd,InRe},A,Vertex_{2nd→1})>Angle(Incident_{2nd,InRe},A,Vertex_{2nd→2}),ceil(((Angle(Incident_{2nd,InRe},A,Vertex_{2nd→1})+0)/(π-2 θ_{2nd,Incident}))),

    tir ∧ plzdtyA ∧ Angle(
      
      Incident_{2nd,InRe},A,Vertex_{2nd→2})>Angle(Incident_{2nd,InRe},A,Vertex_{2nd→1}),ceil(((Angle(Incident_{2nd,InRe},A,Vertex_{2nd→2})+0)/(π-2 θ_{2nd,Incident}))),

    tir ∧ plzdtyB ∧ Angle(

      Incident_{2nd,InRe},B,Vertex_{2nd→1})>Angle(Incident_{2nd,InRe},B,Vertex_{2nd→2}),ceil(((Angle(Incident_{2nd,InRe},B,Vertex_{2nd→1})+0)/(π-2 θ_{2nd,Incident}))),

    tir ∧ plzdtyB ∧ Angle(

      Incident_{2nd,InRe},B,Vertex_{2nd→2})>Angle(Incident_{2nd,InRe},B,Vertex_{2nd→1}),ceil(((Angle(Incident_{2nd,InRe},B,Vertex_{2nd→2})+0)/(π-2 θ_{2nd,Incident})))

    )

  δ=If(tir ∧ plzdtyA ∧ Angle(Incident_{2nd,InRe},A,Vertex_{2nd→1})>Angle(Incident_{2nd,InRe},A,Vertex_{2nd→2}),ceil(((Angle(Incident_{2nd,InRe},A,Vertex_{2nd→1}))/(π-2 θ_{2nd,Incident}))),tir ∧ plzdtyA ∧ Angle(Incident_{2nd,InRe},A,Vertex_{2nd→2})>Angle(Incident_{2nd,InRe},A,Vertex_{2nd→1}),ceil(((Angle(Incident_{2nd,InRe},A,Vertex_{2nd→2}))/(θ_{2nd,Incident}))),tir ∧ plzdtyB ∧ Angle(Incident_{2nd,InRe},B,Vertex_{2nd→1})>Angle(Incident_{2nd,InRe},B,Vertex_{2nd→2}),ceil(((Angle(Incident_{2nd,InRe},B,Vertex_{2nd→1}))/(θ_{2nd,Incident}))),tir ∧ plzdtyB ∧ Angle(Incident_{2nd,InRe},B,Vertex_{2nd→2})>Angle(Incident_{2nd,InRe},B,Vertex_{2nd→1}),ceil(((Angle(Incident_{2nd,InRe},B,Vertex_{2nd→2}))/(θ_{2nd,Incident}))))